vale/code/arch/x64/Vale.X64.Bytes_Semantics.fst
@@ -106,10 +106,10 @@ let same_mem_get_heap_val128 ptr mem1 mem2 =
 through execution *)
 
 let update_operand_flags_same_domains (dst:operand64) (v:nat64) (s_orig s:machine_state) : Lemma
-  (let s1 = update_operand_preserve_flags'' dst v s_orig s in
+  (let s1 = update_operand64_preserve_flags'' dst v s_orig s in
   Set.equal (Map.domain s.ms_mem) (Map.domain s_orig.ms_mem) ==>
   Set.equal (Map.domain s.ms_mem) (Map.domain s1.ms_mem))
-  [SMTPat (update_operand_preserve_flags'' dst v s_orig s)]
+  [SMTPat (update_operand64_preserve_flags'' dst v s_orig s)]
   =
   FStar.Pervasives.reveal_opaque (`%valid_addr64) valid_addr64;
   match dst with
@@ -117,28 +117,28 @@ let update_operand_flags_same_domains (dst:operand64) (v:nat64) (s_orig s:machin
   | _ -> ()
 
 let update_operand_same_domains (dst:operand64) (ins:ins) (v:nat64) (s:machine_state) : Lemma
-  (let s1 = update_operand' dst ins v s in
+  (let s1 = update_operand64' dst ins v s in
   Set.equal (Map.domain s.ms_mem) (Map.domain s1.ms_mem))
-  [SMTPat (update_operand' dst ins v s)]
+  [SMTPat (update_operand64' dst ins v s)]
   =
   update_operand_flags_same_domains dst v s s
 
 #set-options "--z3rlimit 20"
 let update_operand128_flags_same_domains (o:operand128) (v:quad32) (s_orig s:machine_state) : Lemma
-  ( let s1 = update_mov128_op_preserve_flags'' o v s_orig s in
+  ( let s1 = update_operand128_preserve_flags'' o v s_orig s in
     Set.equal (Map.domain s.ms_mem) (Map.domain s_orig.ms_mem) ==>
     Set.equal (Map.domain s.ms_mem) (Map.domain s1.ms_mem))
-  [SMTPat (update_mov128_op_preserve_flags'' o v s_orig s)]
+  [SMTPat (update_operand128_preserve_flags'' o v s_orig s)]
   =
   FStar.Pervasives.reveal_opaque (`%valid_addr128) valid_addr128;
   Vale.Def.Opaque_s.reveal_opaque update_heap128_def;
   match o with
-  | OMem (m, _) ->
+  | OMem (m, t) ->
       let ptr = eval_maddr m s_orig in
       if not (valid_addr128 ptr s.ms_mem) then ()
       else
         // This line is unusued, but needed
-        let s1 = update_mem128 ptr v s in
+        let s1 = update_mem128_and_taint ptr v s t in
         reveal_opaque update_heap32_def;
         let mem = update_heap32 ptr v.lo0 s.ms_mem in
         assert (Set.equal (Map.domain s.ms_mem) (Map.domain mem));
@@ -154,10 +154,10 @@ let update_operand128_flags_same_domains (o:operand128) (v:quad32) (s_orig s:mac
 
 #push-options "--max_fuel 0 --max_ifuel 1 --initial_ifuel 1"
 let update_operand_flags_same_unspecified (dst:operand64) (v:nat64) (s_orig s:machine_state) : Lemma
-  (let s1 = update_operand_preserve_flags'' dst v s_orig s in
+  (let s1 = update_operand64_preserve_flags'' dst v s_orig s in
   Set.equal (Map.domain s.ms_mem) (Map.domain s_orig.ms_mem) ==>
   (forall x.{:pattern (s.ms_mem.[x])} not (Map.contains s1.ms_mem x && Map.contains s.ms_mem x) ==> s1.ms_mem.[x] == s.ms_mem.[x]))
-  [SMTPat (update_operand_preserve_flags'' dst v s_orig s)]
+  [SMTPat (update_operand64_preserve_flags'' dst v s_orig s)]
   =
   match dst with
   | OMem _ -> reveal_opaque update_heap64_def
@@ -165,9 +165,9 @@ let update_operand_flags_same_unspecified (dst:operand64) (v:nat64) (s_orig s:ma
 #pop-options
 
 let update_operand_same_unspecified (dst:operand64) (ins:ins) (v:nat64) (s:machine_state) : Lemma
-  (let s1 = update_operand' dst ins v s in
+  (let s1 = update_operand64' dst ins v s in
   forall x.{:pattern (s.ms_mem.[x])} not (Map.contains s1.ms_mem x && Map.contains s.ms_mem x) ==> s1.ms_mem.[x] == s.ms_mem.[x])
-  [SMTPat (update_operand' dst ins v s)]
+  [SMTPat (update_operand64' dst ins v s)]
   =
   update_operand_flags_same_unspecified dst v s s
 
@@ -184,20 +184,20 @@ let update_heap32_same_unspecified (ptr:int) (v:nat32) (h:heap) : Lemma
   reveal_opaque update_heap32_def
 
 let update_operand128_flags_same_unspecified (o:operand128) (v:quad32) (s_orig s:machine_state) : Lemma
-  (let s1 = update_mov128_op_preserve_flags'' o v s_orig s in
+  (let s1 = update_operand128_preserve_flags'' o v s_orig s in
   Set.equal (Map.domain s.ms_mem) (Map.domain s_orig.ms_mem) ==>
   (forall x.{:pattern (s.ms_mem.[x])} not (Map.contains s1.ms_mem x && Map.contains s.ms_mem x) ==> s1.ms_mem.[x] == s.ms_mem.[x]))
-  [SMTPat (update_mov128_op_preserve_flags'' o v s_orig s)]
+  [SMTPat (update_operand128_preserve_flags'' o v s_orig s)]
   =
   FStar.Pervasives.reveal_opaque (`%valid_addr128) valid_addr128;
   Vale.Def.Opaque_s.reveal_opaque update_heap128_def;
   match o with
-  | OMem (m, _) ->
+  | OMem (m, t) ->
       let ptr = eval_maddr m s_orig in
       if not (valid_addr128 ptr s.ms_mem) then ()
       else
         // This line is unusued, but needed
-        let s1 = update_mem128 ptr v s in
+        let s1 = update_mem128_and_taint ptr v s t in
         update_heap32_same_unspecified ptr v.lo0 s.ms_mem;
         let mem = update_heap32 ptr v.lo0 s.ms_mem in
         update_heap32_same_unspecified (ptr+4) v.lo1 mem;
@@ -243,28 +243,26 @@ let rec instr_write_outputs_bs_domains
 #set-options "--z3rlimit 30 --max_ifuel 1"
 
 let eval_ins_bs_domains (ins:ins) (s0:machine_state) : Lemma
-  (let s1 = run (untainted_eval_ins ins) s0 in
+  (let s1 = run (machine_eval_ins_st ins) s0 in
   Set.equal (Map.domain s0.ms_mem) (Map.domain s1.ms_mem))
   =
-  let s1 = run (untainted_eval_ins ins) s0 in
+  let s1 = run (machine_eval_ins_st ins) s0 in
   match ins with
   | _ -> assert (Set.equal (Map.domain s0.ms_mem) (Map.domain s1.ms_mem))
 
 #set-options "--z3rlimit 30"
 
 let eval_ins_domains i s0 =
-  let s = run (check (taint_match_ins i s0.ms_memTaint s0.ms_stackTaint)) s0 in
-  eval_ins_bs_domains i s
+  eval_ins_bs_domains i s0
 
 #set-options "--z3rlimit 30 --max_ifuel 2"
 let eval_ins_bs_same_unspecified (ins:ins) (s0:machine_state) : Lemma
-  (let s1 = run (untainted_eval_ins ins) s0 in
+  (let s1 = run (machine_eval_ins_st ins) s0 in
    forall x. not (Map.contains s1.ms_mem x) ==> s1.ms_mem.[x] == s0.ms_mem.[x])
   =
   ()
 #set-options "--z3rlimit 30 --max_ifuel 1"
 
 let eval_ins_same_unspecified i s0 =
-  let s0 = {s0 with ms_trace = []} in
-  let s = run (check (taint_match_ins i s0.ms_memTaint s0.ms_stackTaint)) s0 in
+  let s = {s0 with ms_trace = []} in
   eval_ins_bs_same_unspecified i s
