vale/code/arch/x64/Vale.X64.InsLemmas.fsti
@@ -17,15 +17,15 @@ val lemma_valid_taint64_operand (m:maddr) (t:taint) (s:va_state) : Lemma
   (ensures taint_at s.memTaint (eval_maddr m s) == t)
   [SMTPat (eval_maddr m s); SMTPat (OMem #int #reg (m, t))]
 
-val lemma_valid_taint_match64 (o:operand64) (s:state) : Lemma
+val lemma_valid_src_operand64_and_taint (o:operand64) (s:state) : Lemma
   (requires valid_operand o s)
-  (ensures S.taint_match o s.memTaint s.stackTaint (state_to_S s))
-  [SMTPat (S.taint_match o s.memTaint s.stackTaint (state_to_S s))]
+  (ensures S.valid_src_operand64_and_taint o (state_to_S s))
+  [SMTPat (S.valid_src_operand64_and_taint o (state_to_S s))]
 
-val lemma_valid_taint_match128 (o:operand128) (s:state) : Lemma
+val lemma_valid_src_operand128_and_taint (o:operand128) (s:state) : Lemma
   (requires valid_operand128 o s)
-  (ensures S.taint_match128 o s.memTaint s.stackTaint (state_to_S s))
-  [SMTPat (S.taint_match128 o s.memTaint s.stackTaint (state_to_S s))]
+  (ensures S.valid_src_operand128_and_taint o (state_to_S s))
+  [SMTPat (S.valid_src_operand128_and_taint o (state_to_S s))]
 
 [@instr_attr]
 let rec make_instr_t_args (args:list instr_operand) : Type0 =
